src/coq/dot/meta_binding.v
@@ -2,5 +2,12 @@ Set Implicit Arguments.
 Require Import syntax_binding.
 Require Import Metatheory LibTactics_sf support.
 
-Lemma open_lc_decl_ident: forall d t, lc_decl d -> open_decl_cond d t d. Admitted.
+Lemma open_lc_decl_ident: forall d t, lc_decl d -> open_decl_cond d t d. Proof. Admitted.
 Lemma open_lc_is_noop : forall T x, lc_tp T -> T = T ^tp^ x. Proof. Admitted.
+
+(*
+*** Local Variables: ***
+*** coq-prog-name: "coqtop" ***
+*** coq-prog-args: ("-emacs-U" "-I" "../metalib") ***
+*** End: ***
+*)  
