src/coq/dot/meta_pres_tp.v
@@ -2,63 +2,92 @@ Set Implicit Arguments.
 Require Import List.
 Require Import syntax_binding theory.
 Require Import Metatheory LibTactics_sf support.
-Require Import meta_pres_subst meta_weakening meta_inversion meta_binding meta_regular.
+Require Import meta_pres_subst meta_weakening meta_inversion meta_binding meta_regular meta_decls meta_quality meta_path_eq.
 Require Import Coq.Program.Equality.
-
-
-Lemma red_pres_path: forall s t t' s' E' T q DS q', 
-  E' |== s' -> path t -> s |~ t ~~> t' ~| s' -> E' |= t' ~: T @ q -> E' |= T ~< DS @ q' -> DS <> nil
-    -> path t'.
-Proof.
-  introv HStoTp Hpath Hred Htp HX. generalize dependent q'. generalize dependent q. generalize dependent T. generalize dependent DS. induction Hred; intros; inverts Hpath; eauto. inverts H2 (*value v*); auto.
-
-  destruct (invert_typing_lam HStoTp Htp) as [? [? [? [? [? [? [? HSubFun]]]]]]]. 
-  set (expands_sub_safe HStoTp HSubFun HX) as HXF. destruct HXF as [qq HXF']. set (invert_expands_fun HXF'). tauto.
-  apply path_sel. 
-
-  destruct (invert_typing_sel HStoTp Htp) as [T' [q1 [HT [DS' [q2 [HX' [D [HIn [S [Hopen [q3 HSub]]]]]]]]]]].
-  eapply IHHred; eauto. unfold not. intros. induction DS'; eauto. inversion H0.
-Qed.
 
 
 Section Preservation.
 (* mostly reusable boilerplate for the mutual induction: *)
-  Let P0_ (E: env) (q: quality) (t: tm) (T: tp) (H: E  |=  t ~: T  @ q) := forall t' s s', 
-    E  |== s -> s  |~  t ~~> t'  ~| s' ->
-      (exists E', 
-        E' |== s' 
-          /\ dom (fst E) [<=] dom (fst E') 
-          /\ exists q', E' |=  t' ~: T @ q').
+  Let P0_ (E_s: env) (q: quality) (t: tm) (T: tp) (H: E_s |=  t ~: T  @ q) := forall E t' s s', E_s = (E, s) -> 
+      E |== s -> s  |~  t ~~> t'  ~| s' -> (E |== s' /\ exists q', (E, s') |=  t' ~: T @ q').  
   Let P1_ (E : env) (q : quality) (T : tp) (DS : decls) (H: E |= T ~< DS @ q) := True.
   Let P2_ (E : env) (q : quality) (T T' : tp) (H: E |= T ~<: T' @ q) := True.
   Let P3_ (e : env) (q : quality) (d d0 : decl) (H: sub_decl e q d d0) := True.
   Let P4_ (e : env) (t t0 : tm) (H: path_eq e t t0) := True.
   Let P5_ (e : env) (H: wf_env e) := True.
-  Let P6_ (c : ctx) (H: wf_ctx c) := True.
-  Let P7_ (c : ctx) (p : pex) (H: wf_pex c p) := True.
-  Let P8_ (e : env) (t : tp) (H: wf_tp e t) := True.
-  Let P9_ (e : env) (d : decl) (H: wf_decl e d) := True.
+  Let P6_ (e : env) (t : tp) (H: wf_tp e t) := True.
+  Let P7_ (e : env) (d : decl) (H: wf_decl e d) := True.
 Lemma preservation : preservation. 
 Proof. unfold preservation. 
-  mutind_typing P0_ P1_ P2_ P3_ P4_ P5_ P6_ P7_ P8_ P9_.
-  (*var*) intros ? ? ? ? ? ? ? ? Hred. inversion Hred.
-  (*ref*) intros ? ? ? ? ? ? ? ? Hred. inversion Hred.
-  (*sel*) intros H IH HT'X _ Hin HopenD. introv Hsto_tp Hred.
+  mutind_typing P0_ P1_ P2_ P3_ P4_ P5_ P6_ P7_; try solve [intros until s'; intros _ _ HRed; inverts HRed | idtac ].
+  (*sel*) intros H IH HT'X _ Hin HopenD. introv ? Hsto_tp Hred. subst.
     inverts Hred as. 
-    SCase "red_sel". introv Hsto_wf Ha_in_sto HInArgs Hl_in_args.
-      exists E. splits; [eauto | unfold AtomSetImpl.Subset; eauto | idtac]. (* store doesn't change*)
+    SCase "red_sel". introv Hsto_wf Ha_in_sto HInArgs Hl_in_args. 
+      split; auto.  rename t' into v. clear IH.
 
 (* invert store typing to get well-formedness of the selected constructor argument *)
-      inverts Hsto_tp as. intros _ [HEnvStoDom Hsto_tp']. 
-      destruct (Hsto_tp' a Tc ags DS Ha_in_sto) as [ags0 [HAgsEq [HXPex [HTcConc [HAtpTc [HTcX [L Hwf_args]]]]]]]. clear Hsto_tp'.
-      pick fresh x for L. set (Hwf_args x Fr) as Hwfargs. inverts Hwfargs as. intros HDupA [HSameDomAgsDecls Hwf_args']. clear Hwf_args. subst.
-      destruct (Hwf_args' l D Hin) as [_ HWfD0]. unfold open_decl in HWfD0. 
+      inversion Hsto_tp as [_ Hsto_tp']. 
+      destruct (Hsto_tp' a Tc ags Ha_in_sto) as [ags0 [HAgsEq [HTcConc [HDupA [DS0 [HTcX [HSameDomAgsDecls [L Hwf_args]]]]]]]]. clear Hsto_tp'.
+      pick fresh x for L. set (Hwf_args x Fr) as Hwfargs.  subst.
+
+(* XXX TODO
+  H : (E0, s') |= ref a ~: T' @ q1
+destruct (invert_typing_ref E0 s' a T' q1 H) as [Ta [ags' [Ha_in_sto' [qa HSubTa]]]]
+  Ha_in_sto' : binds a (Ta, ags') s'
+  HSubTa : (E0, s') |= Ta ~<: T' @ q
+
+  Hsto_wf : wf_store s'
+  Ha_in_sto : binds a (Tc, ags0 ^args^ ref a) s'
+set binds_uniq_wf_store (Ha_in_sto' Ha_in_sto Ha_in_sto). subst.
+
+  HSubTa : (E0, s') |= Tc ~<: T' @ q
+  HT'X : (E0, s') |= T' ~< DS @ q2
+apply expands_sub_safe
+  HTcX : (E0, s') |= Tc ~< DS @ (q & q2)
+  HTcConc : concrete Tc
+  Hin : LabelMapImpl.binds l D DS
+destruct invert_expands_concrete
+  HTcX' : (E0, s') |= Tc ~< DS' @ precise
+  sub_decls DS' DS
+
+  HTcX : (E0, s') |= Tc ~< DS0 @ precise
+destruct expands_precise_concrete_unique
+
+  DS' = DS0
+
+  sub_decls DS0 DS
+  Hin : LabelMapImpl.binds l D DS
+apply sub_decls_pres_binds
+
+  Hin0 : LabelMapImpl.binds l D' DS0
+  sub_decl D' D
+*)
+
+      assert (exists D', LabelMapImpl.binds l D' DS0 /\ exists q, sub_decl (E0, s') q D' D) as [D' [Hin' [qd HSubD]]].
+      destruct (invert_typing_ref H) as [Ta [ags' [Ha_in_sto' [qa HSubTa]]]].
+      set (binds_unique _ a (Tc, ags0 ^args^ ref a) (Ta, ags') s' Ha_in_sto Ha_in_sto' (invert_wf_store_uniq Hsto_wf)) as HH. injsubst HH.
+      assert ( exists q3, (E0, s') |= Ta ~< DS @ q3) as HTaX by (eapply expands_sub_safe; eauto).
+      destruct HTaX as [qxta HTaX].
+      destruct (invert_expands_concrete HTaX HTcConc) as [DSa [HXTaP [qsdp Hsubdecls]]].
+      assert ((E0, s') |= DS0 <:DS<: DS) as HSubDecls by (eapply quality_soundness; eauto).
+(*
+Hin : LabelMapImpl.binds l D DS
+HSubDecls : (E0, s') |= DS0 <:DS<: DS
+====
+Hin : LabelMapImpl.binds l D' DS0
+sub_decl D' D
+*)
+      destruct HSubDecls as [qsd HSubDecls]. 
+      destruct (sub_decls_pres_binds l D Hin HSubDecls) as [D0 [qsd0 [Hin0 HSubD0]]].
+      exists D0. splits; eauto.
+      destruct (Hwfargs l D' Hin') as [_ HWfD0]. unfold open_decl in HWfD0. 
 
 (* figure out what the declaration's type was opened to: replace D by decl_tm ?? *)
-      inverts HopenD as; intros Hapath HDopena; [auto | destruct Hapath; apply path_ref]. induction D; inverts HDopena. simpl in HWfD0. 
+      inverts HopenD as; intros Hapath HDopena; [auto | destruct Hapath; apply path_ref]. induction D; inverts HDopena. inverts HSubD. simpl in HWfD0. rename t into T. 
 
+      
 (* finally get at the typing judgment for the declaration *)      
-      destruct (HWfD0 ({0 ~tp> x}t) eq_refl) as [v' [HInArgs' [_ HWfDTp]]]. change ({0 ~tp> x}t) with (t ^tp^ x) in HWfDTp. clear Hwf_args' HWfD0.
+      destruct (HWfD0 ({0 ~tp> x}T1) eq_refl) as [v' [HInArgs' [_ HWfDTp]]]. change ({0 ~tp> x}T1) with (T1 ^tp^ x) in HWfDTp. clear HWfD0. subst.
  
 (* commute opening with label lookup *)
 (*
@@ -66,10 +95,19 @@ Proof. unfold preservation.
   HInArgs : LabelMapImpl.binds l t' (LabelMapImpl.map (open_rec_tm 0 a) ags0)
   HInArgs': LabelMapImpl.binds l v' ags0
 *)
-      assert (t' = ({0 ~> (ref a)}v')) by (eapply LabelMapImpl.binds_unique; eauto; [
+      assert (v = ({0 ~> (ref a)}v')) by (eapply LabelMapImpl.binds_unique; eauto; [
       unfold open_args; apply (LabelMapImpl.binds_map_2 tm tm (open_rec_tm 0 (ref a)) l v' ags0 HInArgs') |
       apply LabelMapImpl.uniq_map_2; eauto]). subst.
-      change ({0 ~> (ref a)}v') with (v' ^^ (ref a)). change ({0 ~tp> (ref a)}t) with (t ^tp^ (ref a)). rename t into T.
+      change ({0 ~> (ref a)}v') with (v' ^^ (ref a)). change ({0 ~tp> (ref a)}T) with (T ^tp^ (ref a)).
+
+
+(*
+   H4 : (E0, s') |= T1 ~<: T @ qd
+subtyping_regular
+open_lc_is_noop
+*)
+   destruct (regular_subtyping H4) as [_ [HLcT1 HLcT]].
+   rewrite (@open_lc_is_noop T1 x HLcT1) in H4. rewrite (@open_lc_is_noop T x HLcT) in H4.
 
 (* apply the substitution lemma
 
@@ -77,23 +115,35 @@ Proof. unfold preservation.
   ============================
   exists q', E |= v' ^^ a ~: T ^tp^ a @ q'
 *)
-      apply subst_pres_typing with (x := x) (Tx := Tc); eauto.
+
+      apply subst_pres_typing with (x := x) (Tx := Tc); [ 
+        destruct HWfDTp; eexists; eapply typing_sub; eauto |
+        eauto |
+        destruct (regular_expands HTcX) as [HWfE HLcTc]; eexists; eapply typing_ref; eauto]. 
+        eapply weakening_subtyping; eauto. simpl. fsetdec.
 
    SCase "red_sel_tgt". rename t into t0. rename e' into t0'. 
-      intros Hred0. set (@IH t0' s s' Hsto_tp Hred0) as HH. destruct HH as [E' [Hsto_tp' [Hdom [q1' H']]]].
-      exists E'. splits; auto.
+      intros Hred0. set (@IH E0 t0' s s' eq_refl Hsto_tp Hred0) as HH. destruct HH as [Hsto_tp' [q1' H']].
+      split; auto.
       exists (q1' & q2).
      
       (* recreate typing judgement for reduced subterm: apply typing_sel to typing judgement from IH, re-use old expansion *)
 
       inverts HopenD. (* was the self variable replaced by t0 in the typing judgement before reduction? *)
+          assert (path t0'). eapply (red_pres_path Hsto_tp' H3 Hred0); eauto. 
+            eapply weakening_expansion_store; eauto. eapply inversion_red_store_dom; eauto.
+            unfold not. intros HDSnil. induction DS; eauto. inversion HDSnil. (* DS <> nil from In D DS*)
+
+
         (* yep, prove path equivalence t0 == t0' and apply typing_peq *) 
         induction D; unfold open_decl in H0; simpl in H0; inverts H0. rename t into T. change ({0 ~tp> t0}T) with (T ^tp^ t0).
 
-          assert (E' |= sel t0' l ~: T ^tp^ t0' @ q1' & q2). 
+          assert ((E0, s') |= sel t0' l ~: T ^tp^ t0' @ q1' & q2). 
           apply typing_sel with (T' := T') (D := (decl_tm T)) (DS := DS); try assumption.
-          apply weakening_expansion with (E := E); assumption. 
-          apply open_decl_path. 
+          eapply weakening_expansion_store; eauto. eapply inversion_red_store_dom; eauto.
+
+
+          apply open_decl_path; auto.
 (*   
    Hred0 : s |~ t0 ~~> t0' ~| s'
    path t0
@@ -103,12 +153,9 @@ Proof. unfold preservation.
    ====== red_pres_path
    t0' path
 *)
-          eapply (red_pres_path Hsto_tp' H3 Hred0); eauto.
-            apply weakening_expansion with (E := E); eauto. 
-            unfold not. intros HDSnil. induction DS; eauto. inversion HDSnil. (* DS <> nil from In D DS*)
 
           replace (q1' & q2) with  ((q1' & q2) & precise).
-          eapply (typing_sub H0 (sub_tp_path_eq T _)); try assumption. induction qconj; eauto.
+          eapply (typing_sub H0); eauto. eapply sub_tp_path_eq; eauto. 
 (*   Hred0 : s |~ t0 ~~> t0' ~| s'
    path t0
    path t0'
@@ -116,27 +163,31 @@ Proof. unfold preservation.
    ====== red_implies_peq
    peq E' t0 t0'
 *)
+          eapply red_implies_peq; eauto.
+
+          induction qconj; eauto.
+
         (* nope *)
-        apply typing_sel with (T' := T') (D := (decl_tm T)) (DS := DS); auto; [
-          apply weakening_expansion with (E := E); assumption |
-          apply open_lc_decl_ident; assumption].
+        apply typing_sel with (T' := T') (D := (decl_tm T)) (DS := DS); auto.
+          eapply weakening_expansion_store; eauto. eapply inversion_red_store_dom; eauto.
+          apply open_lc_decl_ident; assumption.
 
-  (*sub*) intros HT IHT HSub _. introv. intros HStoTp HRed. destruct (IHT t' s s' HStoTp HRed) as [E' [HStoTp' [HDom HT']]]. 
-    exists E'. inversion HT' as [q' HT'']. split; try assumption. split; try assumption.
-    eexists. eapply typing_sub; eauto. eapply weakening_subtyping; eauto.
+  (*sub*) intros HT IHT HSub _. introv ? HStoTp HRed. subst. destruct (IHT E0 t' s s' eq_refl HStoTp HRed) as [HStoTp' HT']. 
+    inversion HT' as [q' HT'']. split; try assumption. 
+    eexists. eapply typing_sub; eauto. eapply weakening_subtyping_store; eauto; eapply inversion_red_store_dom; eauto.
 
-Focus.
-
-  (*app*) intros HTFun IHTFun HTArg IHTArg. introv. intros HStoTp HRed. inverts HRed.
-    SCase "red_beta". exists E. split; auto. split; auto. unfold AtomSetImpl.Subset. auto. clear IHTArg IHTFun.
+  (*app*) intros HTFun IHTFun HTArg IHTArg. introv ? HStoTp HRed. subst. inverts HRed.
+    SCase "red_beta". split; auto. clear IHTArg IHTFun.
       destruct (invert_typing_lam HStoTp HTFun) as [q0 [L [Tr' [HT [HWf [HLcT [? Hsubfun]]]]]]]. 
-      assert (exists T1', exists T2', subsumes_fun_tp (tp_fun Ta Tr) T1' T2' /\ (exists q, E |= T1' ~<: T @ q /\ (exists q0, E |= Tr' ~<: T2' @ q0))) as [T1' [T2' [HSFT [qa [HSubArg [qr HSubRes]]]]]]. 
-        destruct (invert_subtyping_fun) as [_ InvSubFun]. 
-        eapply (InvSubFun E x (tp_fun T Tr') (tp_fun Ta Tr)  Hsubfun); eauto.
+      destruct (invert_subtyping_fun) as [_ InvSubFun]. 
+      assert (exists T1', exists T2', subsumes_fun_tp (tp_fun Ta Tr) T1' T2' 
+                /\ (exists q, (E0, s') |= T1' ~<: T @ q 
+                /\ (exists q0, (E0, s') |= Tr' ~<: T2' @ q0))) as [T1' [T2' [HSFT [qa [HSubArg [qr HSubRes]]]]]]. 
+        eapply (InvSubFun (E0, s') x (tp_fun T Tr') (tp_fun Ta Tr)  Hsubfun); eauto.
         unfold not. intros. inverts H.
      inverts HSFT.
 
-     assert (exists q, E |= t ^^ ta ~: Tr' ^tp^ ta @ q).
+     assert (exists q, (E0, s') |= t ^^ ta ~: Tr' ^tp^ ta @ q).
       pick fresh z for L. set (HT z Fr) as HT'. 
       apply subst_pres_typing with (x := z) (Tx := T); eauto. 
       replace (Tr' ^tp^ z) with (Tr'); [idtac | apply open_lc_is_noop; eauto]. eexists; eauto.
@@ -145,22 +196,107 @@ Focus.
     destruct H. eexists; eapply typing_sub; eauto.
 
     SCase "red_app_fun".
-      destruct (IHTFun e' s s' HStoTp H5) as [E' [HStoTp' [HDom [qf' HTFun']]]].
-      exists E'. split; eauto. split; eauto. exists qf'. 
-        assert (exists q, E' |= ta ~: Ta @ q) as [qa HTa] by (eapply weakening_typing; eauto). 
+      destruct (IHTFun E0 e' s s' eq_refl HStoTp H5) as [? [qf' HTFun']].
+      split; auto. exists qf'. 
+        assert (exists q, (E0, s') |= ta ~: Ta @ q) as [qa HTa] by (eapply weakening_typing_store; eauto; eapply inversion_red_store_dom; eauto).
         eapply typing_app; eauto.
 
     SCase "red_app_arg".
-      destruct (IHTArg e' s s' HStoTp H5) as [E' [HStoTp' [HDom [qa' HTArg']]]].
-      exists E'. split; eauto. split; eauto. 
-        assert (exists q, E' |= tf ~: tp_fun Ta Tr @ q) as [qf HTf] by (eapply weakening_typing; eauto). 
+      destruct (IHTArg E0 e' s s' eq_refl HStoTp H5) as [? [qa' HTArg']].
+      split; auto. 
+        assert (exists q, (E0, s') |= tf ~: tp_fun Ta Tr @ q) as [qf HTf] by (eapply weakening_typing_store; eauto; eapply inversion_red_store_dom; eauto).
         exists qf. eapply typing_app; eauto.
 
-  (* lam *) intros HTpBody IHBody HLcT HWfFunT _. introv. intros HStoTp HRed. inverts HRed.
-  (* new *) intros HWfTc _ HConcTc HTcX _ IHt HLcT. introv. intros HStoTp HRed. inverts HRed.
+  (* new *) intros HWfTc _ HConcTc HTcX _ HArgsUniq HDomDsEqArgs HArgsWf HT IHt. introv ? HStoTp HRed. subst. inverts HRed.
+   destruct (regular_expands HTcX) as [HWfE HLcTc].
+   split. 
+     SCase "extended store is well-typed in extended env".
+     unfold typing_store. Focus. splits.
+       apply wf_store_cons_tp; auto.
+(*
+TP:
+  HArgsUniq : LabelMapImpl.uniq args
+  H7 : forall (v' : tm), LabelMapImpl.binds l v' args -> value (v' ^^ ref a)
+  H : LabelMapImpl.binds l v (args ^args^ ref a)
+  =====
+  value v
+
+remember (open_rec_tm 0 (ref a)) as f. 
+
+  f = {0 -> (ref a)}
+  HArgsUniq : uniq args
+  H7 : forall v', binds l v' args -> value (f v')
+  H : binds l v ((map f) args)
+  =====
+  value v
+
+  H : binds l v ((map f) args)
+
+destruct (binds_map_3 H) as [v' H']
+
+  H': binds l v' args
+
+set (binds_map_2 f H') as H''
+
+  H'': binds l (f v') ((map f) args)
+
+set (binds_unique H H'' HArgsUniq) as Heqvv'
+
+  Heqvv' : v = (f v')
+
+rewrite Heqvv'
+
+rewrite Heqf. apply H7 with (l := l); auto.
+
+*)
+
+     intros. unfold open_args in H. remember (open_rec_tm 0 (ref a)) as f. 
+     destruct (binds_map_3 l v f args H) as [v' H'].
+     set (LabelMapImpl.binds_map_2 tm tm f l v' args H') as H''.
+     set (LabelMapImpl.binds_unique tm l v (f v') (LabelMapImpl.map f args) H H'' (LabelMapImpl.uniq_map_2 tm tm f args HArgsUniq)) as Heqvv'.
+     rewrite Heqvv'.
+     rewrite Heqf. apply H7 with (l := l); auto.
+
+     (* split off the new binding, the rest of the store is ok by HStoTp *)
+       simpl. introv. rewrite binds_cons_iff. apply or_ind; revert a0 Tc0 argsRT.
+       (* the new binding *) introv [HEq HEq']. subst. injsubst HEq'. Focus.
+       exists args. splits; eauto. exists ds. split.
+       eapply weakening_expansion_store; eauto. simpl. fsetdec.
+       split; auto.
+       exists L. intros x Fr. introv HBindsL. destructs (HArgsWf x Fr l d HBindsL).
+       split.
+         intros. destruct (H U T0 H1). eexists; eapply weakening_subtyping_store; eauto. simpl. fsetdec.
+         intros. destruct (H0 T0 H1). destruct H3 as [HBinds [HVal [qx HTx]]]. exists x0. splits; eauto. 
+         eapply weakening_typing_store; [eauto | eapply HTx]. simpl. fsetdec.
+       (* invert HStoTp and apply weakening_???_store *)
+       introv Ha_in_sto. 
+      inversion HStoTp as [_ Hsto_tp']. destruct (Hsto_tp' a0 Tc0 argsRT Ha_in_sto) as [ags0 [HAgsEq [HTcConc [HDupA [DS0 [HTcX' [HSameDomAgsDecls [L' Hwf_args]]]]]]]]. 
+      exists ags0. splits; eauto. exists DS0. split.
+       eapply weakening_expansion_store; eauto. simpl. fsetdec.
+       split; auto.
+       exists L'. intros x Fr. introv HBindsL. destructs (Hwf_args x Fr l d HBindsL).
+       split.
+         intros. destruct (H U T0 H1). eexists; eapply weakening_subtyping_store; eauto. simpl. fsetdec.
+         intros. destruct (H0 T0 H1). destruct H3 as [HBinds [HVal [qx HTx]]]. exists x0. splits; eauto. 
+         eapply weakening_typing_store; [eauto | eapply HTx]. simpl. fsetdec.
+
+     SCase "opening up the body with (ref a) is well-typed in E'".
+       pick fresh x for L. set (HT x Fr) as HTAss0.
+       destruct (regular_typing HTAss0) as [HWFE [_ HLcT]].
+       assert (exists q,  ctx_bind (E0,  [(a, (Tc, args ^args^ ref a))] ++ s) x Tc |= t ^ x ~: T @ q) as HTpAss. eapply weakening_typing_store; eauto.  simpl. fsetdec. 
+       replace (T) with (T ^tp^ x) in HTpAss; [idtac | rewrite <- open_lc_is_noop; eauto].
+       replace (T) with (T ^tp^ (ref a)); [idtac | rewrite <- open_lc_is_noop; eauto]. 
+       apply subst_pres_typing with (x := x) (Tx := Tc); eauto. 
+       eexists; eapply typing_ref; eauto.
+       eapply weakening_wf_env_store; eauto.
+Qed.
+
+End Preservation.
+(*
+   unfold typing_store.
+
    set (E' := ( a ~ Tc ++ fst E, extract_pex a args ++ snd E)).
    assert (dom (fst E)[<=]dom (fst E')) by (simpl; fsetdec).
-   destruct (regular_expands HTcX) as [HWfE HLcTc]. inversion HWfE.
    assert (wf_env E') as HWfE'. 
      eapply wf_env_; eauto. eapply wf_ctx_cons_tp; eauto. 
        rewrite <- H3. simpl. auto. 
@@ -169,8 +305,7 @@ Focus.
        inversion HStoTp. rewrite <- H3. simpl. auto. admit.
 (*
   wf_store s
-  forall (l : label) (v : tm),
-  LabelMapImpl.binds l v args -> value (v ^^ ref a)
+  forall (l : label) (v : tm), LabelMapImpl.binds l v args -> value (v ^^ ref a)
   a `notin` dom s
   wf_pex G P
   dom G [=] dom s
@@ -186,23 +321,8 @@ Focus.
 *)
    exists E'. 
      split; [idtac | split; [simpl; fsetdec | idtac]].
-     SCase "bigger store is well-typed in bigger env".
-     simpl. admit.
-     SCase "opening up the body with (ref a) is well-typed in E'".
-      pick fresh x for L. set (IHt x Fr) as IHT'. 
-      simpl. 
-      unfold ctx_bind in IHT'. 
-      assert (exists q,  ([(x, Tc)] ++ fst E', snd E') |= t ^ x ~: T @ q) as HTpAss. apply weakening_typing with (E := ([(x, Tc)] ++ fst E, snd E)) (q := q). simpl. fsetdec. apply IHT'.
-      replace (T) with (T ^tp^ x) in HTpAss; [idtac | rewrite <- open_lc_is_noop; eauto]. 
-      replace (T) with (T ^tp^ (ref a)); [idtac | rewrite <- open_lc_is_noop; eauto]. 
-      apply subst_pres_typing with (x := x) (Tx := Tc); eauto. 
-      eexists; eapply typing_ref; eauto.
-        (* ctx_binds E' a Tc *) unfold ctx_binds. simpl. auto.
 
-Qed.
-
-End Section.
-
+*)
 (*
 *** Local Variables: ***
 *** coq-prog-name: "coqtop" ***
