src/coq/dot/meta_regular.v
@@ -1,0 +1,22 @@
+Set Implicit Arguments.
+Require Import List.
+Require Import syntax_binding theory.
+Require Import Metatheory LibTactics_sf support.
+Require Import meta_pres_subst.
+Require Import Coq.Program.Equality.
+
+
+Lemma regular_expands: forall E T DS q,  E |= T ~< DS @ q -> wf_env E /\ lc_tp T. Admitted.
+Lemma regular_subtyping: forall E T T' q,  E |= T ~<: T' @ q -> wf_env E /\ lc_tp T /\ lc_tp T'. Admitted.
+Lemma regular_typing: forall E t T q,  E |= t ~: T @ q -> wf_env E /\ lc_tm t /\ lc_tp T. Admitted.
+
+(*Lemma regular_typing: forall E t T q,  E |= t ~: T @ q -> wf_env E /\ lc_tm t /\ lc_tp T. Admitted.
+Lemma regular_wf: forall E T,  wf_tp E T -> lc_tp T. Admitted.*)
+
+
+(*
+*** Local Variables: ***
+*** coq-prog-name: "coqtop" ***
+*** coq-prog-args: ("-emacs-U" "-I" "../metalib") ***
+*** End: ***
+*)  
