src/coq/dot/meta_weakening.v
@@ -7,10 +7,20 @@ Require Import Coq.Program.Equality.
 
 (* todo weaken to allow quality to vary *)
 
-(* TODO: bindings in E and E' must be checked for new-well-formedness  -- do we need to preserve the quality? *)
+(* TODO: bindings in E and E' must be checked for new-well-formedness  -- need to preserve the quality *)
 Lemma weakening_expansion: forall E E' T DS q,  dom (fst E)[<=]dom (fst E') -> E |= T ~< DS @ q -> E' |= T ~< DS @ q. Admitted.
-
-(* TODO: bindings in E and E' must be checked for new-well-formedness  -- do we need to preserve the quality? *)
 Lemma weakening_subtyping: forall E E' S T q,  dom (fst E)[<=]dom (fst E') -> E |= S ~<: T @ q -> E' |= S ~<: T @ q. Admitted.
 
+Lemma weakening_expansion_store: forall E s s' T DS q,  dom s [<=] dom s' -> (E, s) |= T ~< DS @ q -> (E, s') |= T ~< DS @ q. Admitted.
+Lemma weakening_subtyping_store: forall E s s' S T q,  dom s [<=] dom s' -> (E, s) |= S ~<: T @ q -> (E, s') |= S ~<: T @ q. Admitted.
+Lemma weakening_typing_store: forall E s s' t T q,  dom s [<=] dom s' -> (E, s) |= t ~: T @ q -> exists q, (E, s') |= t ~: T @ q. Admitted.
+Lemma weakening_wf_env_store: forall E s a Tc args,  wf_env (E, s) -> wf_env (E, a ~ (Tc, args) ++ s). Admitted.
 Lemma weakening_typing: forall E E' t T q,  dom (fst E)[<=]dom (fst E') -> E |= t ~: T @ q -> exists q, E' |= t ~: T @ q. Admitted.
+
+
+(*
+*** Local Variables: ***
+*** coq-prog-name: "coqtop" ***
+*** coq-prog-args: ("-emacs-U" "-I" "../metalib") ***
+*** End: ***
+*)  
